AbstractInterpretation.v
@@ -1,0 +1,125 @@
+(** Formal Reasoning About Programs <http://adam.chlipala.net/frap/>
+  * Chapter 7: Abstract Interpretation and Dataflow Analysis
+  * Author: Adam Chlipala
+  * License: https://creativecommons.org/licenses/by-nc-nd/4.0/ *)
+
+Require Import Frap Imp.
+
+Set Implicit Arguments.
+
+
+Record absint := {
+  Typeof :> Set;
+  (* This [:>] notation lets us treat any [absint] as its [Typeof],
+   * automatically. *)
+  Top : Typeof;
+  (* The least precise element of the lattice *)
+  Join : Typeof -> Typeof -> Typeof;
+  (* Least upper bound of two elements *)
+  Represents : nat -> Typeof -> Prop
+  (* Which lattice elements represent which numbers? *)
+}.
+
+Definition absint_sound (a : absint) :=
+  (* [Top] really does cover everything. *)
+  (forall n, a.(Represents) n a.(Top))
+
+  (* [Join] really does return an upper bound. *)
+  /\ (forall x y n, a.(Represents) n x
+                    -> a.(Represents) n (a.(Join) x y))
+  /\ (forall x y n, a.(Represents) n y
+                    -> a.(Represents) n (a.(Join) x y)).
+
+Definition astate (a : absint) := fmap var a.
+Definition astates (a : absint) := fmap cmd (astate a).
+
+Inductive compatible a (ss : astates a) (v : valuation) (c : cmd) : Prop :=
+| Compatible : forall s,
+  ss $? c = Some s
+  -> (forall x n xa, v $? x = Some n
+                     -> s $? x = Some xa
+                     -> a.(Represents) n xa)
+  -> compatible ss v c.
+
+Definition merge_astate a : astate a -> astate a -> astate a :=
+  merge (fun x y =>
+           match x with
+           | None => None
+           | Some x' =>
+             match y with
+             | None => None
+             | Some y' => Some (a.(Join) x' y')
+             end
+           end).
+
+Definition merge_astates a : astates a -> astates a -> astates a :=
+  merge (fun x y =>
+           match x with
+           | None => y
+           | Some x' =>
+             match y with
+             | None => Some x'
+             | Some y' => Some (merge_astate x' y')
+             end
+           end).
+
+Inductive oneStepClosure a : astates a -> astates a -> Prop :=
+| OscNil :
+  oneStepClosure $0 $0
+| OscCons : forall ss c s ss' ss'',
+  (forall v c' v', step (v, c) (v', c')
+    -> compatible ss' v' c')
+  -> oneStepClosure ss ss''
+  -> oneStepClosure (ss $+ (c, s)) (merge_astates ss' ss'').
+
+Inductive interpret a : astates a -> astates a -> Prop :=
+| InterpretDone : forall ss,
+  (forall v c, compatible ss v c
+               -> forall v' c', step (v, c) (v', c')
+                                -> compatible ss v' c')
+  -> interpret ss ss
+
+| InterpretStep : forall ss ss' ss'',
+  oneStepClosure ss ss'
+  -> interpret (merge_astates ss ss') ss''
+  -> interpret ss ss''.
+
+Lemma interpret_sound' : forall v c a (ss ss' : astates a),
+  interpret ss ss'
+  -> ss $? c = Some $0
+  -> invariantFor (trsys_of v c) (fun p => compatible ss' (fst p) (snd p)).
+Proof.
+  induct 1; simplify.
+
+  apply invariant_induction; simplify; propositional; subst; simplify.
+
+  econstructor.
+  eassumption.
+  simplify.
+  equality.
+
+  cases s; cases s'; simplify.
+  eapply H.
+  eassumption.
+  assumption.
+
+  apply IHinterpret.
+  unfold merge_astates; simplify.
+  rewrite H1.
+  cases (ss' $? c); trivial.
+  f_equal.
+  maps_equal.
+  unfold merge_astate; simplify.
+  trivial.
+Qed.
+
+Theorem interpret_sound : forall v c a (ss : astates a),
+  interpret ($0 $+ (c, $0)) ss
+  -> invariantFor (trsys_of v c) (fun p => compatible ss (fst p) (snd p)).
+Proof.
+  simplify.
+  eapply interpret_sound'.
+  eassumption.
+  simplify.
+  trivial.
+Qed.
